\documentclass[fleqn,12pt]{article}

\usepackage[utf8]{inputenc}
\usepackage[T1]{fontenc}
\usepackage{mathtools} %loads amsmath
\usepackage{amsthm}
\usepackage{amsfonts}
\usepackage{amsmath}
\usepackage{amssymb}
\usepackage{graphicx}
\usepackage{tikz}
\usetikzlibrary{arrows,automata,positioning}
\usepackage{arydshln}
\usepackage{stmaryrd}
\usepackage{pdflscape}
\usepackage{rotating}
\usepackage[margin=2cm]{geometry}
\usepackage[font=small,labelfont=bf,tableposition=top]{caption}
\usepackage{ebproof}

\tikzset{initial text={}}

\usepackage{fancyhdr}
\setlength{\headheight}{26pt}
\pagestyle{fancy}
\lhead{Static Program Analysis WS 2016/17 -- Series 08 \\ \small{Igor Dudschenko (296764), Oliver Westphal (358321)}}
\rhead{}

\newcommand\dbrackets[1]{\llbracket #1 \rrbracket}

\setlength{\parindent}{0cm}
\newcommand\note[1]{\textcolor{red}{#1}}

\begin{document}
\section*{Exercise 1}
\subsection*{a)}
To show:
$$\alpha(\bot_L) = \bot_M$$
Proof:
$$\alpha \text{ is uniquely dermined by $\gamma$ as follows: } \alpha(l) = \bigsqcap \{m \in M | l \sqsubseteq_L \gamma(m)\}$$
$$\Rightarrow  \alpha(\bot_L) = \bigsqcap \{m \in M | \bot_L \sqsubseteq_L \gamma(m) \}\} = \bigsqcap M = \bot_M$$
$$\Rightarrow \alpha(\bot_L) = \bot_M$$

\subsection*{b)}
To show:
$$\gamma(\bot_M) = \bot_L$$
Proof:
$$\gamma \text{ is uniquely dermined by $\alpha$ as follows: } \gamma(m) = \bigsqcup \{l \in L | \alpha(l) \sqsubseteq_M m\}$$
$$\Rightarrow \gamma(\bot_M) = \bigsqcup \{l \in L | \alpha(l) \sqsubseteq_M \bot_M\}$$
$$\Rightarrow \gamma(\bot_M) = \bot_L$$

\subsection*{c)}
To show:
$$\alpha \circ \gamma \circ \alpha = \alpha$$
Proof:
$$\forall l \in L: l \sqsubseteq_{L} \gamma(\alpha(l)) \text{ and: } \forall m \in M: \alpha(\gamma(m)) \sqsubseteq_{M} m$$
$$\Rightarrow \alpha(l) \sqsubseteq_M \alpha(\gamma(\alpha(l))) \sqsubseteq_M \alpha(l)$$
Thus:
$$\alpha \circ \gamma \circ \alpha = \alpha$$
%To show:
%$$\alpha \circ \gamma \circ \alpha = \alpha$$
%Proof:
%$$\forall l \in L: l \sqsubseteq_{L} \gamma(\alpha(l)) \text{ and: } \forall m \in M: \alpha(\gamma(m)) \sqsubseteq_{M} m$$
%$$\Rightarrow \alpha \sqsubseteq_M \alpha \circ (\gamma \circ \alpha) \text{ (monotonicity of $\alpha$)}$$
%And:
%$$\Rightarrow (\alpha \circ \gamma) \circ \alpha \sqsubseteq_M \alpha \text{ (monotonicity of $\alpha$)}$$
%Thus:
%$$\alpha \circ \gamma \circ \alpha = \alpha$$
\subsection*{d)}
To show:
$$\gamma \circ \alpha \circ \alpha = \gamma$$
Proof:
$$\forall l \in L: l \sqsubseteq_{L} \gamma(\alpha(l)) \text{ and: } \forall m \in M: \alpha(\gamma(m)) \sqsubseteq_{M} m$$
$$\Rightarrow \gamma(m) \sqsubseteq_L \gamma(\alpha(\gamma(m))) \sqsubseteq_L \gamma(m)$$
Thus:
$$\gamma \circ \alpha \circ \alpha = \gamma$$
%To show:
%$$\gamma \circ \alpha \circ \gamma = \gamma$$
%Proof:
%$$\forall l \in L: l \sqsubseteq_{L} \gamma(\alpha(l)) \text{ and: } \forall m \in M: \alpha(\gamma(m)) \sqsubseteq_{M} m$$
%$$\Rightarrow \gamma \sqsubseteq_L (\gamma \circ \alpha) \circ \gamma \text{ (monotonicity of $\gamma$)}$$
%And:
%$$\Rightarrow \gamma \circ (\alpha \circ \gamma) \sqsubseteq_L \gamma \text{ (monotonicity of $\gamma$)}$$
%Thus:
%$$\gamma \circ \alpha \circ \gamma = \gamma$$
\section*{Exercise 2}

\subsection*{1)}
Extend the execution function introduced in the lecture by:\\
(push)
\begin{prooftree}
	\Infer0[]{val_{\sigma}(s) = i_0 i_1 \dots i_n}
	\Infer1[]{<s.push(a),\sigma> \rightarrow <\downarrow, \sigma [s \mapsto val_{\sigma}(a) \cdot i_0 i_1 \dots i_n]>}
\end{prooftree}
\\
(pop)
\begin{prooftree}
	\Infer0[]{val_\sigma(s)=i_0 i_1 \dots i_n}
	\Infer1[]{<s.pop(),\sigma> \rightarrow <\downarrow,\sigma [s \mapsto i_1 \dots i_n] ]>}
\end{prooftree}
\subsection*{2)}
Given:
\begin{enumerate}
	\item $L = 2^{\mathbb{Z^{*}} \times \mathbb{Z^{*}}}$
	\item $M_1 = 2^{\{H,S\}}$
	\item $M_2 = 2^{\mathbb{Z}}$
	\item $M_1 \times M_2 = 2^{\{H,S\}} \times 2^{\mathbb{Z}}$
\end{enumerate}
Required for $(\alpha,\gamma)$ is a product of:
	\begin{enumerate}
		\item $(\alpha_1,\gamma_1)$ between $L$ and $M_1$
		\item $(\alpha_2,\gamma_2)$ between $L$ and $M_2$
	\end{enumerate}
\section*{Exercise 3}
\subsection*{a)}

\subsection*{b)}

\subsection*{c)}

\subsection*{d)}

\end{document}
